src/threadpool/ctrace.v
@@ -3,7 +3,7 @@ From Paco Require Import paco.
 From Paco Require Import paco2.
 From stdpp Require Import list.
 From iris.itree.threadpool Require Import handler interleaving.
-From iris.itree Require Import axioms itree.
+From iris.itree Require Import axioms itree trace.
 Import Coq.Logic.ClassicalChoice.
 
 Section scheduler.
@@ -401,84 +401,6 @@ Section is_ctrace.
     Transitive is_postfix.
   Admitted.
 End is_ctrace.
-
-Inductive trace (E : Type → Type) (R : Type) :=
-  | TRet (r : R)
-  | TVis (A : Type) (e : E A) (a : A) (k : trace E R)
-  | TVisEmpty (A : Type) (e : E A)
-  | TCut.
-
-Arguments TRet {_ _}.
-Arguments TVis {_ _}.
-Arguments TVisEmpty {_ _}.
-Arguments TCut {_ _}.
-
-Section is_trace.
-  Context {E : Type → Type} {R : Type}.
-
-  Inductive is_trace_
-    : trace E R
-    → itree' E R
-    → Prop :=
-  | is_TRet r :
-    is_trace_ (TRet r) (RetF r)
-  | is_TVis tr' A (e : E A) a k :
-    is_trace_ tr' (observe (k a)) →
-    is_trace_ (TVis A e a tr') (VisF e k)
-  | is_TVisEmpty A (f : A → Empty_set) (e : E A) k :
-    is_trace_ (TVisEmpty A e) (VisF e k)
-  | is_TCut t :
-    is_trace_ TCut t
-  | trace_skip_tau tr t' :
-    is_trace_ tr (observe t') →
-    is_trace_ tr (TauF t').
-
-  Definition is_trace (tr : trace E R) (t : itree E R) : Prop :=
-    is_trace_ tr (observe t).
-
-  Local Instance is_trace_eutt_unilateral :
-    Proper (pointwise_relation (trace E R) (eutt (=) ==> impl)) is_trace.
-  Proof.
-    intros tr t1 t2 Heqit Htr.
-    rewrite /is_trace. rewrite /is_trace in Htr.
-    remember (observe t1) as ot1. remember (observe t2) as ot2.
-    revert t1 t2 ot2 Heqot1 Heqot2 Heqit. induction Htr as [r|tr' A e a k Htr IH|A f e k|t|tr t' Htr IH]; intros t1 t2 ot2 Heqot1 Heqot2 Heqit.
-    - punfold Heqit. rewrite /eqit_ in Heqit. remember (observe t1) as ot1. destruct Heqot2.
-      induction Heqit as [r1 r2| | | | ot1 t2' _ _ IH ]; try discriminate.
-      * injection Heqot1 as ->. destruct REL. constructor.
-      * constructor. by apply IH.
-    - punfold Heqit. rewrite /eqit_ in Heqit. remember (observe t1) as ot1. destruct Heqot2.
-      induction Heqit as [ | | B e' k1 k2 REL | | ot1 t2' _ _ IH' ]; try discriminate.
-      * simplify_K. simplify_K. constructor. apply IH with (t1 := k1 a) (t2 := k2 a); try done.
-        pclearbot. apply REL.
-      * constructor. by apply IH'.
-    - punfold Heqit. rewrite /eqit_ in Heqit. remember (observe t1) as ot1. destruct Heqot2.
-      induction Heqit as [ | | B e' k1 k2 REL | | ot1 t2' _ _ IH' ]; try discriminate.
-      * simplify_K. simplify_K. by constructor.
-      * constructor. by apply IH'.
-    - punfold Heqit. rewrite /eqit_ in Heqit. remember (observe t1) as ot1. destruct Heqot2.
-      induction Heqit as [ | | B e' k1 k2 REL | | ot1 t2' _ _ IH' ]; try discriminate; constructor.
-    - apply IH with (t1 := t') (t2 := t2); eauto.
-      transitivity (Tau t'). { by apply eqit_inv_Tau_l. }
-      pfold. rewrite /eqit_. simpl. rewrite Heqot1. punfold Heqit.
-  Qed.
-  Global Instance is_trace_eutt :
-    Proper (pointwise_relation (trace E R) (eutt (=) ==> (↔))) is_trace.
-  Proof.
-    intros tr t1 t2 Heqit. split; by apply is_trace_eutt_unilateral.
-  Qed.
-End is_trace.
-
-Class AnswerEqDecision (E : Type → Type) :=
-  is_AnswerEqDecision A : E A → EqDecision A.
-Print RelDecision.
-Print Decision.
-
-Program Definition equal `{AnswerEqDecision E} {A : Type} (e : E A) (a a' : A) : {a = a'} + {a ≠ a'} :=
-  @decide (a = a') _.
-Next Obligation.
-  intros E Hdec A e a a'. by apply is_AnswerEqDecision.
-Qed.
 
 Fixpoint sequencify {E R} (tr : ctrace E R) : trace E (R + last_thread_killed) :=
   match tr with
